---
title: "MathJax Test"
author: NenkaLab
date: 2017-12-03 17:24
category: Test
tags: ["Test"]
---
#### MathJax Test! <br>
\forall x \in X, \quad \exists y \leq \epsilon <br>
\alpha, \Alpha, \beta, \Beta, \gamma, \Gamma, \pi, \Pi, \phi, \varphi, \mu, \Phi <br>
\cos (2\theta) = \cos^2 \theta - \sin^2 \theta <br>
\lim_{x \to \infty} \exp(-x) = 0 <br>
a \bmod b <br>
x \equiv a \pmod{b} <br>
k_{n+1} = n^2 + k_n^2 - k_{n-1} <br>
n^{22} <br>
f(n) = n^5 + 4n^2 + 2 |_{n=17} <br>
\frac{n!}{k!(n-k)!} = \binom{n}{k} <br>
\frac{\frac{1}{x}+\frac{1}{y}}{y-z} <br>
%running fraction with slash - requires math mode.
^3/_7 <br>
\newcommand*\rfrac[2]{{}^{#1}\!/_{#2}}

\rfrac{3}{7} <br>
Take $\sfrac{1}{2}$ cup of sugar, \dots
 
  3\times\sfrac{1}{2}=1\sfrac{1}{2}
 
<br>
Take ${}^1/_2$ cup of sugar, \dots
 
  3\times{}^1/_2=1{}^1/_2
  <br>
$x^\frac{1}{2}$ % no error <br>
\begin{equation}
  x = a_0 + \cfrac{12356616316}{a_3 
          + \cfrac{16565}{a_3 
          + \cfrac{165465465}{a_9 + \cfrac{1131321}{a_7} } } }
\end{equation} <br>
\begin{equation}
\frac{
    \begin{array}[b]{r}
      \left( x_1 x_2 \right)\\
      \times \left( x'_1 x'_2 \right)
    \end{array}
  }{
    \left( y_1y_2y_3y_4 \right)
  }
\end{equation} <br>
\sqrt{\frac{a}{b}} <br>
\sqrt[n]{1+x+x^2+x^3+\dots+x^n} <br>
% New definition of square root:
% it renames \sqrt as \oldsqrt
\let\oldsqrt\sqrt
% it defines the new \sqrt in terms of the old one
\def\sqrt{\mathpalette\DHLhksqrt}
\def\DHLhksqrt#1#2{%
\setbox0=\hbox{$#1\oldsqrt{#2\,}$}\dimen0=\ht0
\advance\dimen0-0.2\ht0
\setbox2=\hbox{\vrule height\ht0 depth -\dimen0}%
{\box0\lower0.4pt\box2}} <br>
\usepackage{letltxmacro}
\makeatletter
\let\oldr@@t\r@@t
\def\r@@t#1#2{%
\setbox0=\hbox{$\oldr@@t#1{#2\,}$}\dimen0=\ht0
\advance\dimen0-0.2\ht0
\setbox2=\hbox{\vrule height\ht0 depth -\dimen0}%
{\box0\lower0.4pt\box2}}
\LetLtxMacro{\oldsqrt}{\sqrt}
\renewcommand*{\sqrt}[2][\ ]{\oldsqrt[#1]{#2} }
\makeatother


$\sqrt[a]{b} \quad \oldsqrt[a]{b}$ <br>
\sum_{i=1}^{10} t_i <br>
\displaystyle\sum_{i=1}^{10} t_i <br>
\int_0^\infty \mathrm{e}^{-x}\,\mathrm{d}x <br>
\sum_{\substack{
   0<i<m \\
   0<j<n
  }} 
 P(i,j) <br>
\int\limits_a^b <br>
\usepackage[intlimits]{amsmath} <br>
( a ), [ b ], \{ c \}, | d |, \| e \|,
\langle f \rangle, \lfloor g \rfloor,
\lceil h \rceil, \ulcorner i \urcorner <br>
\left(\frac{x^2}{y^3}\right) <br>
P\left(A=2\middle|\frac{A^2}{B}>4\right) <br>
\left\{\frac{x^2}{y^3}\right\} <br>
\left.\frac{x^3}{3}\right|_0^1 <br>
( \big( \Big( \bigg( \Bigg( <br>
\frac{\mathrm d}{\mathrm d x} \left( k g(x) \right) <br>
\frac{\mathrm d}{\mathrm d x} \big( k g(x) \big) <br>
x \in [-1,1] <br>
x \in {[-1,1]} <br>
x \in {[{-1},1]} <br>
\[
 \begin{matrix}
  a & b & c \\
  d & e & f \\
  g & h & i
 \end{matrix}
\] <br>
\begin{matrix}
  -1 & 3 \\
  2 & -4
 \end{matrix}
 =
 \begin{matrix*}[r]
  -1 & 3 \\
  2 & -4
 \end{matrix*} <br>
A_{m,n} = 
 \begin{pmatrix}
  a_{1,1} & a_{1,2} & \cdots & a_{1,n} \\
  a_{2,1} & a_{2,2} & \cdots & a_{2,n} \\
  \vdots  & \vdots  & \ddots & \vdots  \\
  a_{m,1} & a_{m,2} & \cdots & a_{m,n} 
 \end{pmatrix} <br>
\begin{array}{c|c}
  1 & 2 \\ 
  \hline
  3 & 4
 \end{array} <br>
M = \begin{bmatrix}
       \frac{5}{6} & \frac{1}{6} & 0           \\[0.3em]
       \frac{5}{6} & 0           & \frac{1}{6} \\[0.3em]
       0           & \frac{5}{6} & \frac{1}{6}
     \end{bmatrix} <br>
M = \bordermatrix{~ & x & y \cr
                  A & 1 & 0 \cr
                  B & 0 & 1 \cr} <br>
A matrix in text must be set smaller:
$\bigl(\begin{smallmatrix}
a&b \\ c&d
\end{smallmatrix} \bigr)$
to not increase leading in a portion of text. <br>
50 apples \times 100 apples = lots of apples^2 <br>
50 \text{apples} \times 100 \text{apples} 
 = \text{lots of apples}^2 <br>
50 \text{ apples} \times 100 \text{ apples}
 = \text{lots of apples}^2 <br>
50 \textrm{ apples} \times 100
 \textbf{ apples} = \textit{lots of apples}^2 <br>
\boldsymbol{\beta} = (\beta_1,\beta_2,\dotsc,\beta_n) <br>
\pm <br>
\mp <br>
\[ f(n) =
  \begin{cases}
    n/2       & \quad \text{if } n \text{ is even}\\
    -(n+1)/2  & \quad \text{if } n \text{ is odd}
  \end{cases}
\] <br>
\int y \mathrm{d}x <br>
\int y\, \mathrm{d}x <br>
\int y\: \mathrm{d}x <br>
\int y\; \mathrm{d}x <br>
\left(
    \begin{array}{c}
      n \\
      r
    \end{array}
  \right) = \frac{n!}{r!(n-r)!} <br>
\left(\!
    \begin{array}{c}
      n \\
      r
    \end{array}
  \!\right) = \frac{n!}{r!(n-r)!} <br>
\newcommand{\dd}{\mathop{}\,\mathrm{d}} <br>
\begin{equation}
   C^i_j = {\textstyle \sum_k} A^i_k B^k_j
\end{equation} <br>
\newcommand{\tsum}[1]{{\textstyle \sum_{#1}}} <br>
\usepackage{amsmath}
